finished work on some basic primitives for merging sums, need to go back to looking at syntax and semantics in light of these new abstractions

Prism/Sum_Merge_Id.thy
@@ -1,11 +1,22 @@
-theory Sum_Merge_Id imports Sum_Merge
+theory Sum_Merge_Id imports Sum_Merge Prism_Id
 
 begin
 
-(* the plan:
 
-- define "prod-like" types
-- show "prod-like" types are iso. to products
-- show "prod-like" types are Product_Merge *)
+abbreviation sum_merge_id_parms :: "('t, 't, 't) sum_merge_parms" where
+"sum_merge_id_parms \<equiv>
+  \<lparr> prism1 = prism_id_parms
+  , prism2 = prism_id_parms \<rparr>"
+
+locale Sum_Merge_Id_Spec
+
+sublocale Sum_Merge_Id_Spec \<subseteq> Sum_Merge_Spec "sum_merge_id_parms"
+  apply(simp add:Sum_Merge_Spec_def) apply(safe)
+   apply(rule_tac Prism_Id_Itp.Prism_Spec_axioms)
+  apply(unfold_locales, auto)
+  done
+
+interpretation Sum_Merge_Id_Itp : Sum_Merge_Id_Spec
+  done
 
 end
