Prism/Prism_Id.thy
@@ -1,0 +1,19 @@
+theory Prism_Id imports "Prism"
+
+begin
+
+abbreviation prism_id_parms :: "('a, 'a) prism_parms" where
+"prism_id_parms \<equiv> 
+  \<lparr> cases = (\<lambda> a . Inl a)
+  , inj = id \<rparr>"
+
+locale Prism_Id_Spec
+
+sublocale Prism_Id_Spec \<subseteq> Prism_Spec "prism_id_parms :: ('t, 't) prism_parms"
+  apply(unfold_locales) apply(auto)
+  done
+
+interpretation Prism_Id_Itp : Prism_Id_Spec
+  done
+
+end
