Prism/Prism_Swap.thy
@@ -1,0 +1,36 @@
+theory Prism_Swap imports Prism
+begin
+
+abbreviation prism_swap_parms ::
+  "('a + 'b, 'c) prism_parms \<Rightarrow> ('b + 'a, 'c) prism_parms" where
+"prism_swap_parms p \<equiv>
+  \<lparr> cases =
+    (\<lambda> c . case (cases p c) of
+            Inl (Inl a) \<Rightarrow> Inl (Inr a)
+            | Inl (Inr b) \<Rightarrow> Inl (Inl b)
+            | Inr c \<Rightarrow> Inr c)
+  , inj = (\<lambda> ba .
+    (case ba of
+      Inl b \<Rightarrow> inj p (Inr b)
+      | Inr a \<Rightarrow> inj p (Inl a))) \<rparr>"
+
+locale Prism_Swap_Spec' =
+  fixes Prism_Swap_parms :: "('a + 'b, 'c) prism_parms"
+
+locale Prism_Swap_Spec = Prism_Swap_Spec' +
+  P : Prism_Spec "Prism_Swap_parms"
+
+sublocale Prism_Swap_Spec \<subseteq> Prism_Spec "prism_swap_parms Prism_Swap_parms"
+  apply(insert P.Prism_Spec_axioms)
+  apply(unfold_locales)
+  apply(auto split: sum.splits)
+             apply(auto simp add:P.Prism_Spec_axioms Prism_Spec_def)
+       apply(drule_tac x = c in spec) apply(drule_tac x = c in spec) apply(auto)
+      apply(drule_tac x = c in spec) apply(drule_tac x = c in spec) apply(auto)
+     apply(drule_tac x = c in spec) apply(drule_tac x = c in spec) apply(auto)
+    apply(drule_tac x = c in spec) apply(drule_tac x = c in spec) apply(auto)
+   apply(drule_tac x = c in spec) apply(drule_tac x = c in spec) apply(auto)
+apply(drule_tac x = c in spec) apply(drule_tac x = c in spec) apply(auto)
+  done
+
+end
